theories/logrel/examples/subtyping.v
@@ -1,3 +1,10 @@
+(** This file demonstrates how Löb induction can be used to prove subtyping
+of recursive protocols that combine polymorphism and asynchornous subtyping.
+In pseudo syntax, the subtyping we show is:
+
+     μ rec. ! (X,Y:★) (X ⊸ Y). !X. ?Y. rec
+  <: μ rec. ! (X1,X2:★) (X1 ⊸ bool). !X1. !(X2 ⊸ int). !X2. ?bool. ?int. rec
+*)
 From actris.channel Require Import proofmode proto channel.
 From actris.logrel Require Import subtyping_rules.
 From iris.proofmode Require Import tactics.
@@ -5,32 +12,30 @@ From iris.proofmode Require Import tactics.
 Section basics.
   Context `{heapG Σ, chanG Σ}.
 
-  Definition prot1_aux : (lsty Σ → lsty Σ) :=
-    λ rec, (<!!X Y> TY (X ⊸ Y)%lty ; <!!> TY X;
-           <??> TY Y; rec)%lty.
+  Definition prot1_aux (rec : lsty Σ) : lsty Σ :=
+    <!! X Y> TY (X ⊸ Y); <!!> TY X; <??> TY Y; rec.
   Instance prot1_aux_contractive : Contractive prot1_aux.
   Proof. solve_proto_contractive. Qed.
   Definition prot1 := lty_rec prot1_aux.
 
-  Definition prot1'_aux : (lsty Σ → lsty Σ) :=
-    λ rec, (<!!X Y> TY (X ⊸ Y)%lty ; <!!> TY X;
-           <??> TY Y;
-           <!!X Y> TY (X ⊸ Y)%lty ; <!!> TY X;
-           <??> TY Y; rec)%lty.
+  Definition prot1'_aux (rec : lsty Σ) : lsty Σ :=
+    <!! X Y> TY (X ⊸ Y); <!!> TY X;
+    <??> TY Y;
+    <!! X Y> TY (X ⊸ Y); <!!> TY X;
+    <??> TY Y; rec.
   Instance prot1'_aux_contractive : Contractive prot1'_aux.
   Proof. solve_proto_contractive. Qed.
   Definition prot1' := lty_rec prot1'_aux.
 
-  Definition prot2_aux : (lsty Σ → lsty Σ) :=
-    λ rec, (<!!X> TY (X ⊸ lty_bool)%lty ; <!!> TY X;
-            <!!Y> TY (Y ⊸ lty_int)%lty ; <!!> TY Y;
-            <??> TY lty_bool; <??> TY lty_int; rec)%lty.
+  Definition prot2_aux (rec : lsty Σ) : lsty Σ :=
+    <!! X> TY (X ⊸ lty_bool); <!!> TY X;
+    <!! Y> TY (Y ⊸ lty_int); <!!> TY Y;
+    <??> TY lty_bool; <??> TY lty_int; rec.
   Instance prot2_aux_contractive : Contractive prot2_aux.
   Proof. solve_proto_contractive. Qed.
   Definition prot2 := lty_rec prot2_aux.
 
-  Lemma rec_swap_example :
-    ⊢ prot1 <: prot2.
+  Lemma rec_swap_example : ⊢ prot1 <: prot2.
   Proof.
     iApply (lty_le_trans _ prot1').
     { iLöb as "IH".
@@ -41,22 +46,16 @@ Section basics.
       iIntros (X Y). iExists X, Y. do 3 iModIntro.
       iApply (lty_le_trans with "H1").
       iIntros (X' Y'). iExists X', Y'. do 3 iModIntro.
-      iApply "IH".
-    }
+      iApply "IH". }
     iApply lty_le_rec.
-    iIntros (M1 M2) "#Hrec".
-    iIntros (X). iExists X, lty_bool. iModIntro. iModIntro.
-    iIntros (Y).
-    iApply (lty_le_trans _ (<??> TY lty_bool ; <!!> TY Y ⊸ lty_int ;
-                            <!!> TY Y ; <??> TY lty_int ; M2)); last first.
-    {
-      iApply (lty_le_trans _ (<!!> TY Y ⊸ lty_int ; <??> TY lty_bool ;
-                              <!!> TY Y ; <??> TY lty_int ; M2)).
+    iIntros (S1 S2) "#Hrec".
+    iIntros (X). iExists X, lty_bool. iIntros "!> !>" (Y).
+    iApply (lty_le_trans _ (<??> TY lty_bool; <!!> TY Y ⊸ lty_int;
+                            <!!> TY Y; <??> TY lty_int; S2)); last first.
+    { iApply (lty_le_trans _ (<!!> TY Y ⊸ lty_int; <??> TY lty_bool;
+                              <!!> TY Y; <??> TY lty_int; S2)).
       { iApply lty_le_swap_recv_send. }
-      iModIntro. iApply lty_le_swap_recv_send.
-    }
-    iModIntro. iExists Y, lty_int.
-    by do 3 iModIntro.
+      iModIntro. iApply lty_le_swap_recv_send. }
+    iModIntro. iExists Y, lty_int. by do 3 iModIntro.
   Qed.
-
 End basics.
